src/lib/data/array/Kuiper.IArray.fsti
@@ -89,23 +89,25 @@ val iarray_pts_to
   : slprop
 
 instance
-val is_send_across_global_iarray
+val is_send_iarray_cell
   (#et:Type0)
   (#vw : aiview)
-  (x: iarray et vw { is_global x })
-  (#f : perm)
-  (v : (vw.ait -> GTot et))
-  : is_send_across gpu_of (iarray_pts_to x #f v)
-
-instance
-val is_send_across_global_iarray_cell
-  (#et:Type0)
-  (#vw : aiview)
-  (a: iarray et vw { is_global a })
+  (a : iarray et vw)
+  (vis : visibility { vis_refines vis (visibility_of (core a)) })
   (#f : perm)
   (i : vw.ait)
   (v : et)
-  : is_send_across gpu_of (iarray_pts_to_cell a #f i v)
+  : is_send_across vis (iarray_pts_to_cell a #f i v)
+
+instance
+val is_send_iarray
+  (#et:Type0)
+  (#vw : aiview)
+  (x : iarray et vw)
+  (vis : visibility { vis_refines vis (visibility_of (core x)) })
+  (#f : perm)
+  (v : (vw.ait -> GTot et))
+  : is_send_across vis (iarray_pts_to x #f v)
 
 unfold
 instance has_pts_to (#et:Type0) (#vw : aiview)
