src/lib/data/array/Kuiper.VArray.fsti
@@ -100,25 +100,27 @@ val varray_pts_to
   : slprop
 
 instance
-val is_send_across_global_varray
+val is_send_varray_cell
   (#et:Type0)
   (#st : Type0)
   (#vw : aview et st)
-  (x: varray vw { is_global x })
-  (#f : perm)
-  (v : st)
-  : is_send_across gpu_of (varray_pts_to x #f v)
-
-instance
-val is_send_across_global_varray_cell
-  (#et:Type0)
-  (#st : Type0)
-  (#vw : aview et st)
-  (a : varray vw { is_global a })
+  (a : varray vw)
+  (vis : visibility { vis_refines vis (visibility_of (core a)) })
   (#f : perm)
   (i : vw.iview.ait)
   (v : et)
-  : is_send_across gpu_of (varray_pts_to_cell a #f i v)
+  : is_send_across vis (varray_pts_to_cell a #f i v)
+
+instance
+val is_send_varray
+  (#et:Type0)
+  (#st : Type0)
+  (#vw : aview et st)
+  (x : varray vw)
+  (vis : visibility { vis_refines vis (visibility_of (core x)) })
+  (#f : perm)
+  (v : st)
+  : is_send_across vis (varray_pts_to x #f v)
 
 unfold
 instance has_pts_to (#a:Type) (#st:Type) (#vw : aview a st)
